Dafny/Printer.cs
@@ -834,18 +834,29 @@ namespace Microsoft.Dafny {
           string op;
           int opBindingStrength;
           switch (e.Op) {
+            case UnaryExpr.Opcode.SetChoose:
+              op = "choose";  opBindingStrength = -1;  break;
             case UnaryExpr.Opcode.Not:
               op = "!";  opBindingStrength = 0x60;  break;
             default:
               Contract.Assert(false); throw new cce.UnreachableException();  // unexpected unary opcode
           }
-          bool parensNeeded = opBindingStrength < contextBindingStrength ||
-            (fragileContext && opBindingStrength == contextBindingStrength);
+          if (opBindingStrength == -1) {
+            // print as a function
+            wr.Write(op);
+            wr.Write("(");
+            PrintExpression(e.E);
+            wr.Write(")");
+          } else {
+            // print as an operator
+            bool parensNeeded = opBindingStrength < contextBindingStrength ||
+              (fragileContext && opBindingStrength == contextBindingStrength);
 
-          if (parensNeeded) { wr.Write("("); }
-          wr.Write(op);
-          PrintExpr(e.E, opBindingStrength, false, -1);
-          if (parensNeeded) { wr.Write(")"); }
+            if (parensNeeded) { wr.Write("("); }
+            wr.Write(op);
+            PrintExpr(e.E, opBindingStrength, false, -1);
+            if (parensNeeded) { wr.Write(")"); }
+          }
         }
       
       } else if (expr is BinaryExpr) {
