Util/Emacs/dafny-mode.el
@@ -36,7 +36,7 @@
         "invariant" "decreases"
         )) . font-lock-builtin-face)
    `(,(dafny-regexp-opt '(
-        "assert" "assume" "break" "call" "then" "else" "havoc" "if" "label" "return" "while" "print"
+        "assert" "assume" "break" "call" "choose" "then" "else" "havoc" "if" "label" "return" "while" "print"
         "old" "forall" "exists" "new" "foreach" "in" "this" "fresh" "allocated" "use"
         "match" "case" "false" "true" "null")) . font-lock-keyword-face)
    `(,(dafny-regexp-opt '("array" "array2" "array3" "bool" "int" "object" "set" "seq")) . font-lock-type-face)
